\section*
{Exponential Family}

One can define 
\begin{gather*}
    \text{
    exponential 
    family:}
\quad 
    \condProb 
    {x}{\theta} 
\equiv
    h(x) 
\cdot 
    e^
    {
        \innerProd
        {\theta}
        {\phi} 
    -
        A 
        (\theta) }
        ,
\\
\qq{log partition:}
    A 
    (\theta) 
=
    \log 
    \int _{x \in S}
    \dd{\mu [x]}
    e^
    { \innerProd
      {\theta} {\phi}}
    , 
\qq{features:}
    \phi := 
    \phi (x)
    .
\end{gather*}  

\subsection* 
{Cumulant is convex}
Let us demonstrate 
that $A$ is convex.  
Recall that 
a real function $f$ is convex,  
if 
$$
    f( \lambda x + (1-\lambda) y ) 
\leq
    \lambda f(x) 
+
    (1 - \lambda) f(y)
$$  
for all $x, y \in \mathbb{R}$.

For said task, 
we need Holder's inequality.
For 
$\alpha, \beta 
\in \mathbb{R}$,
that if 
$p^{-1} + q^{-1}  
\overset{!}{=} 1: 
    \innerProd 
    {\alpha} {\beta} 
\leq 
    \norm {\alpha} _{p}
    \cdot 
    \norm {\beta} _{q}
$, where
$$
    \innerProd
    {\alpha}
    {\beta}
=
    \int _{x\in S}
    \dd{\mu[x]}
    \cdot 
    (
    \alpha 
    \beta )
\quad 
    \norm{\alpha _{p}}
\equiv 
    \qty(
        \int _{x\in S}
        \dd{\mu[x]}
        \cdot 
        \alpha ^{p}
    )^{1/p}
\quad 
    \norm{\beta _{q}}
\equiv
    \qty(
        \int _{x\in S}
        \dd{\mu[x]}
        \cdot 
        \beta ^{q}
    )^{1/q}
$$
Then 
\begin{align*}
    A (\theta) 
& \equiv 
    \log 
    \int _{x \in S}
    \dd{\mu [x]}
    e^
    { \innerProd
      {\theta} {\phi}}  
\end{align*} 
Letting 
$  \theta (\lambda) 
= 
   \lambda \theta_{1} 
   + (1 - \lambda) \theta_{2} $,
Cumulant (i.e $A$) 
becomes: 
\begin{align*}
    A (\theta _{\lambda}) 
& =
    \log \int _{x\in S} 
    \mu[ \dd{x} ] 
\cdot 
    e^{
        \innerProd
        { \lambda \theta_{1} 
          + (1 - \lambda) \theta_{2}
        }
        {\phi}
    } 
=
    \log \int _{x\in S} 
    \mu[ \dd{x} ] 
\cdot
    ( e^{
            \innerProd
            { \theta_{1} }
            {\phi} } ) 
    ^{\lambda} 
    ( e^{
        \innerProd
        { \theta_{2} }
        {\phi} ) } 
    ) 
    ^{1 - \lambda} 
\end{align*}
{\it Holder's Inequality} implies: 
\begin{align*}
        \int _{x\in S} 
        \mu[ \dd{x} ] 
    \cdot
        ( e^{
                \innerProd
                { \theta_{1} }
                {\phi} } ) 
        ^{\lambda} 
        ( e^{
            \innerProd
            { \theta_{2} }
            {\phi} ) } 
        ) 
        ^{1 - \lambda} 
& \leq 
( 
        \int _{x\in S} \mu[ \dd{x} ] 
        \cdot
    (
        e^ 
        { \innerProd
        { \theta_{1} } {\phi}  
        }
    )  
    ^{\lambda / \lambda}
) 
^{\lambda} 
\cdot 
( 
        \int _{x\in S} \mu[ \dd{x} ] 
        \cdot
    (
        e^ 
        {  \innerProd
           { \theta_{2} } {\phi}  
        }
    )  
    ^{ (1 - \lambda ) 
       ( 1 - \lambda)^{-1}
     }
) 
^{1 - \lambda} 
\\ 
& \leq 
( 
        \int _{x\in S} \mu[ \dd{x} ] 
        \cdot
        e^ 
        { \innerProd
        { \theta_{1} } {\phi}  
        }
)  
^{\lambda} 
\cdot 
( 
        \int _{x\in S} \mu[ \dd{x} ] 
        \cdot
        e^ 
        {  \innerProd
           { \theta_{2} } {\phi}  
        }
) 
^{(1 - \lambda)} 
\end{align*}
Since $\log$ is
monotonically increasing 
on $\theta \in \mathbb{R}$,
the inequality propagates 
toward the cumulant:
\begin{gather*}
    \log 
    \int _{x\in S} 
    \mu[ \dd{x} ] 
\cdot
    ( e^{
            \innerProd
            { \theta_{1} }
            {\phi} } ) 
    ^{\lambda} 
    ( e^{
        \innerProd
        { \theta_{2} }
        {\phi} ) } 
    ) 
    ^{1 - \lambda} 
\leq 
    \log 
( 
        \int _{x\in S} \mu[ \dd{x} ] 
        \cdot
        e^ 
        { \innerProd
        { \theta_{1} } {\phi}  
        }
)  
^{\lambda} 
\cdot 
( 
        \int _{x\in S} \mu[ \dd{x} ] 
        \cdot
        e^ 
        {  \innerProd
           { \theta_{2} } {\phi}  
        }
) 
^{(1 - \lambda)} 
\\ 
    A (\theta _{\lambda})
\leq 
    \lambda  \cdot 
    \log 
    ( 
        \int _{x\in S} \mu[ \dd{x} ] 
        \cdot
        e^ 
        { \innerProd
        { \theta_{1} } {\phi}  
        }
    )   
+ 
    (1 - \lambda)  \cdot  
    \log 
    ( 
        \int _{x\in S} \mu[ \dd{x} ] 
        \cdot
        e^ 
        {  \innerProd
           { \theta_{2} } {\phi}  
        }
    ) 
\leq 
    \lambda \cdot A (\theta _{1})
    + (1 - \lambda) 
\cdot 
    A (\theta _{2})
\end{gather*}
So $A$ is {\it convex}.


